---
dificulty: 5
rating: 8
---

[comment]: # (two-sides:: true)
$$
\sum{|p(i)-i|} = (\pm 1)+(\pm 1)+(\pm 2)+(\pm 2)+...+(\pm n)+(\pm n)
$$

Exactly $n$ of them are $+$, and the others are $-$.

$\sum{|p(i)-i|}$ gets the maximum when highest $n$ numbers take $+$ sign and lowest $n$ numbers take $-$ sign.

So, the maximum value is

$$
\begin{align}
&(-1)+(-1)+(-2)+(-2)+...+(-\frac{n-1}{2})+(-\frac{n-1}{2}) \\
&+(-\frac{n+1}{2})+(\frac{n+1}{2}) \\
&+\frac{n+3}{2}+\frac{n+3}{2}+...+n+n \\
&= \frac{n^{2}-1}{2}\tag{1}
\end{align}
$$

Let

$$
\begin{eqnarray}
\begin{cases}
L := \{1, 2, ..., \frac{n-1}{2}\} \\
H := \{\frac{n+3}{2}, ..., n\} \\
\bar{L} := L\cup\{\frac{n+1}{2}\} \\
\bar{H} = H\cup\{\frac{n+1}{2}\}
\end{cases}
\end{eqnarray}
$$

From (1), It's easy to see that $\sum{|p(i)-i|}=\frac{n^{2}-1}{2}$  iff $p(L) \subset \bar{H}$ and $p(H)\subset\bar{L}$.

For brevity, let $k=\frac{n-1}{2}$.

i) $p(L)=H$ and $p(H)\subset\bar{L}$

there are $k!(k+1)!$ cases.

ii) $p(L)\subset\bar{H}$ and $p(H)=L$

there are $k!(k+1)!$ cases.

iii) $p(L)=H$ and $p(H)=L$

there are $k!k!$ cases.

From i), ii), and iii), there are total

$$
2(k!)(k+1)!-k!k! = (2k+1)k!k!
$$

cases.
